theories/base_logic/lib/cancelable_invariants.v
@@ -94,10 +94,9 @@ Section proofs.
   Global Instance into_inv_cinv N γ P : IntoInv (cinv N γ P) N.
   Global Instance elim_inv_cinv p γ E N P P' Q Q' :
     ElimModal True (|={E,E∖↑N}=> (▷ P ∗ cinv_own γ p) ∗ (▷ P ={E∖↑N,E}=∗ True))%I P' Q Q' →
-    ElimInv (↑N ⊆ E) N (cinv N γ P) [cinv_own γ p] P' Q Q'.
+    ElimInv (↑N ⊆ E) N (cinv N γ P) (cinv_own γ p) P' Q Q'.
   Proof.
-    rewrite /ElimInv/ElimModal.
-    iIntros (Helim ?) "(#H1&(Hown&_)&H2)".
+    rewrite /ElimInv /ElimModal. iIntros (Helim ?) "(#H1&Hown&H2)".
     iApply Helim; auto. iFrame "H2".
     iMod (cinv_open E N γ p P with "[#] [Hown]") as "(HP&Hown&Hclose)"; auto. 
     by iFrame.
