theories/base_logic/lib/na_invariants.v
@@ -115,10 +115,9 @@ Section proofs.
   Global Instance elim_inv_na p F E N P P' Q Q':
     ElimModal True (|={E}=> (▷ P ∗ na_own p (F∖↑N)) ∗ (▷ P ∗ na_own p (F∖↑N) ={E}=∗ na_own p F))%I
               P' Q Q' →
-    ElimInv (↑N ⊆ E ∧ ↑N ⊆ F) N (na_inv p N P) [na_own p F] P' Q Q'.
+    ElimInv (↑N ⊆ E ∧ ↑N ⊆ F) N (na_inv p N P) (na_own p F) P' Q Q'.
   Proof.
-    rewrite /ElimInv/ElimModal.
-    iIntros (Helim (?&?)) "(#H1&(Hown&_)&H2)".
+    rewrite /ElimInv /ElimModal. iIntros (Helim (?&?)) "(#H1&Hown&H2)".
     iApply Helim; auto. iFrame "H2".
     iMod (na_inv_open p E F N P with "[#] [Hown]") as "(HP&Hown&Hclose)"; auto. 
     by iFrame.
